Fix SetState proof

external/Goose/github_com/mit_pdos/gokv/simplepb/pb.v
@@ -601,6 +601,7 @@ Definition Server__SetState: val :=
         struct.storeF Server "epoch" "s" (struct.loadF SetStateArgs "Epoch" "args");;
         struct.storeF Server "sealed" "s" #false;;
         struct.storeF Server "nextIndex" "s" (struct.loadF SetStateArgs "NextIndex" "args");;
+        struct.storeF Server "durableNextIndex" "s" (struct.loadF Server "nextIndex" "s");;
         struct.loadF StateMachine "SetStateAndUnseal" (struct.loadF Server "sm" "s") (struct.loadF SetStateArgs "State" "args") (struct.loadF SetStateArgs "NextIndex" "args") (struct.loadF SetStateArgs "Epoch" "args");;
         MapIter (struct.loadF Server "opAppliedConds" "s") (λ: <> "cond",
           lock.condSignal "cond");;
